{
 "cells": [
  {
   "cell_type": "markdown",
   "metadata": {},
   "source": [
    "Having\n",
    "\n",
    " $$\\nabla E = \\rho / \\varepsilon_0 \\text{ , } \\nabla H = 0 \\text{ , } \\nabla \\times E = - \\partial_t B \\text{ , } \\nabla \\times H = J + \\partial_t D \\text{ , } D = \\varepsilon_0 E + P \\text{ , } B = \\mu_0 H + M$$\n",
    "\n",
    " we find\n",
    "\n",
    "\n",
    "$$ \\nabla \\times \\nabla \\times E = \\Delta E - \\nabla (\\nabla E) = - \\partial_t (\\nabla \\times B) $$\n",
    "\n",
    "\n",
    "and having linear materials, as well as no sources present, we find\n",
    "\n",
    "\n",
    "$$ \\Delta E(\\vec{r}, t) + \\mu(\\vec{r}) \\epsilon(\\vec{r}) \\cdot \\partial_t^2 E(\\vec{r}, t) = 0 $$\n",
    "\n",
    "\n",
    "As we assume that $\\vec{E}(x,y,t) = Re[E_z(x,y) \\cdot \\vec{e}_z \\cdot e^{i\\omega t}]$ (ToDo : How can we assume that -  or do we switch to frequency domain?), we find\n",
    "\n",
    "\n",
    "$$ (\\partial_x^2 + \\partial_y^2) E_z + \\mu\\varepsilon(x,y) \\cdot \\omega^2 E_z = 0$$\n",
    "\n",
    "\n",
    "If we additionally assume that the EM-field is propagating in the $x$-direction, we find $\\vec{E}(x,y,t) = Re(E_{z0}(y) \\cdot e^{-i\\gamma x} \\cdot \\vec{e}_z \\cdot e^{-i \\omega t})$ and therefore $ \\partial_x E_z = - i \\gamma E_{z0} \\cdot e^{-i \\gamma x}$ as well as $\\partial_x^2 E_z = - \\gamma^2 E_{z0} \\cdot e^{-i \\gamma x} $ (ToDo : Again how do these assumptions come by?). Plugging in, we find\n",
    "\n",
    "\n",
    "$$ - \\gamma^2 E_{z0} \\cdot e^{-i \\gamma x} + \\partial_y^2 E_{z0} \\cdot e^{-i \\gamma x} + \\mu\\varepsilon(x,y) E_{z0} \\cdot e^{-i \\gamma x} = 0 \\rightarrow \\partial_y^2 E_{z0} + (\\mu\\varepsilon(x,y) - \\gamma^2) E_{z0} = 0 \\rightarrow \\partial_y^2 E_{z0} + k^2 E_{z0} = 0$$\n",
    "\n",
    "\n",
    "where we defined $k^2 = \\mu\\varepsilon \\omega^2 - \\gamma^2$ (ToDo : We need $k^2 > 0$ to get the right solution - can this be violated?). Solving the second order ODE yields\n",
    "\n",
    "\n",
    "$$ E_{z0}(y) = A \\cdot cos(k \\cdot y) + B \\cdot sin(k \\cdot y) $$\n",
    "\n",
    "\n",
    "and combining the results we find\n",
    "\n",
    "\n",
    "$$ E_z(x,y) = A \\cdot cos(k \\cdot y) \\cdot e^{-i \\gamma x} + B \\cdot sin(k \\cdot y) \\cdot e^{-i \\gamma x} $$\n",
    "\n",
    "\n",
    "We will therefore find even and odd modes. As the waveguide is terminated by perfect electric conductors, we have that $E_z = 0 \\ @ \\ y = \\pm d/2$ and find for the even modes\n",
    "\n",
    "$$ cos(k \\pm d/2) = 0 \\rightarrow k \\pm d/2 = \\pm \\pi/2 \\pm 2n\\pi \\rightarrow k = \\frac{(2n + 1)\\pi}{d} \\text{ for } n = 0, 1, \\dots$$\n",
    "\n",
    "and for odd modes\n",
    "\n",
    "$$ sin(k \\pm d/2) = 0 \\rightarrow k \\pm d/2 = n \\pi \\rightarrow k = \\frac{2n \\pi}{d} \\text{ for } n = 1, 2, \\dots$$\n",
    "\n",
    "If we have that $\\gamma \\in \\mathbb{C}$, we find evanescent modes. We want $\\gamma \\in \\mathbb{R}$, we find\n",
    "\n",
    "$$ \\gamma = \\sqrt{\\mu\\varepsilon \\omega^2 - k^2} \\rightarrow w \\geq \\frac{k}{\\sqrt{\\mu\\varepsilon}} = \\frac{kc}{\\eta} = k v $$\n",
    "\n",
    "where we call the smallest $\\omega$ such that the above condition is fullfilled the cut off frequency. We are given the following values\n",
    "\n",
    "$$ d = 0.02 \\ [m] $$\n",
    "\n",
    "$$ \\varepsilon = 8.85 \\cdot 10^{-12} \\ [F/m] $$\n",
    "\n",
    "$$ \\mu = 12.56 \\cdot 10^{-7} \\ [Tm/A] $$\n",
    "\n",
    "Thus, for the fundamental even mode, we find\n",
    "\n",
    "$$ k = \\frac{\\pi}{d} = 157 \\rightarrow f \\geq 7.5 \\cdot 10^9 \\ [Hz] \\leftrightarrow \\text{ First dominant even mode - Single mode propagation range - ToDo }$$\n",
    "\n",
    "We are also given general boundary conditions where the normal vector $\\vec{n}$ is neither in the $x$ or the $y$ direction.\n",
    "\n",
    "---\n",
    "\n",
    "ToDo\n",
    "\n",
    "- Look at General Boundary Conditions - When are they needed\n",
    "- Look at $H$-field derivation\n",
    "\n",
    "---\n",
    "\n",
    "Having $f : \\mathbb{R}^2 \\to \\mathbb{R}, \\vec{x} \\mapsto f(\\vec{x})$ with $- \\nabla (\\alpha \\nabla f) - \\beta f = g \\text{ for } \\vec{x} \\in \\Omega$ subject to $f(\\vec{x}) = p \\text{ for } \\vec{x} \\in \\partial_D \\Omega$ and $\\partial_{\\vec{n}}f(\\vec{x}) = q \\text{ for } \\vec{x} \\in \\partial_N \\Omega$ where $\\partial \\Omega = \\partial_D \\Omega \\cup \\partial_N \\Omega$, with the weightet residual approach (multiply equation by $w$), through integration by parts ($ \\partial_x(fg) = \\partial_x f g + f \\partial_x g$) and using the divergence theorem \n",
    "\n",
    "$$ \\int\\limits_{\\Omega} \\nabla_{\\vec{x}} (\\nabla_{\\vec{x}} f) d\\Omega = \\int\\limits_{\\partial \\Omega} \\nabla_{\\vec{x}} f d\\vec{A} = \\int\\limits_{\\partial \\Omega} \\nabla_{\\vec{n}} f dA = \\int\\limits_{\\partial_N \\Omega} q dA $$\n",
    "\n",
    "where it was used $\\nabla_{\\vec{x}} g \\cdot \\vec{n} = \\nabla_{\\vec{n}} g$, we find\n",
    "\n",
    "$$ \\int\\limits_{\\Omega} \\alpha \\nabla w \\nabla f d\\Omega + \\int\\limits_{\\Omega} \\beta w f d\\Omega - \\int\\limits_{\\Omega} w g d\\Omega - \\int\\limits_{\\partial \\Omega} w \\nabla_{\\vec{n}} f dA = 0 $$\n",
    "\n",
    "by switching to the global representation, we find\n",
    "\n",
    "$$ \\sum\\limits_{e = 1}^{N_e} \\int\\limits_{\\Omega^{(e)}} \\alpha^{(e)} \\nabla w \\nabla f^{(e)} d\\Omega^{(e)} + \\sum\\limits_{e = 1}^{N_e} \\int\\limits_{\\Omega^{(e)}} \\beta^{(e)} w f^{(e)} d\\Omega^{(e)} - \\sum\\limits_{e=1}^{N_e} \\int\\limits_{\\Omega} w g^{(e)} d\\Omega - \\sum\\limits_{\\substack{e \\text{ such that }\\\\ \\partial\\Omega^{(e)} \\in \\partial_N\\Omega}} \\int\\limits_{\\partial \\Omega^{(e)}} w q^{(e)} dA^{(e)} = 0 $$\n",
    "\n",
    "switching to the global notation by using\n",
    "\n",
    "$$ \\sum\\limits_{e=1}^{N_e} f^{(e)} = \\sum\\limits_{n = 1}^{N_n} f_n N_n $$\n",
    "\n",
    "reversing the sums and letting $w = N_m$, we find\n",
    "\n",
    "$$ \\sum\\limits_{n = 1}^{N_n} f_n \\left( \\sum\\limits_{\\substack{e \\in \\\\ Supp(N_n) \\\\ Supp(N_m)}} \\int\\limits_{\\Omega^{(e)}} \\alpha^{(e)} \\nabla N_m \\nabla N_n d\\Omega^{(e)} \\right) + \\sum\\limits_{n=1}^{N_n} f_n \\left( \\sum\\limits_{\\substack{e \\in \\\\ Supp(N_n) \\\\ Supp(N_m)}} \\int\\limits_{\\Omega^{(e)}} \\beta^{(e)} N_m N_n d\\Omega^{(e)} \\right) = \\sum\\limits_{\\substack{e \\in \\\\ Supp(N_m)}} \\left[ \\int\\limits_{\\Omega^{(e)}} N_m g^{(e)} d\\Omega^{(e)} \\right] + \\sum\\limits_{\\substack{e = 1 \\\\ \\partial\\Omega^{(e)} \\in \\partial_N\\Omega \\\\ Supp(N_m)}}  \\left[ \\int\\limits_{\\partial \\Omega^{(e)}} N_m q^{(e)} dA^{(e)} \\right] \\ \\forall \\ m \\in \\{1, 2, \\dots N_n\\}$$\n",
    "\n",
    "evaluating the terms in the brackets for the different nodes leads to\n",
    "\n",
    "$$ A \\vec{f} = \\vec{b} $$\n",
    "\n",
    "subsequently enforcing the boundary conditions results in a solvable LSE yielding the resulting approximated unknown function.\n",
    "\n",
    "---\n",
    "\n",
    "ToDo Matlab\n",
    "\n",
    "- Read in Nodes and Elements (Grid)\n",
    "- What about Boundaries ?\n",
    "- Matrix assembly\n",
    "- Enforcing Boundary Conditions\n",
    "- Plotting\n",
    "\n",
    "---"
   ]
  },
  {
   "cell_type": "markdown",
   "metadata": {},
   "source": []
  }
 ],
 "metadata": {
  "language_info": {
   "name": "python"
  }
 },
 "nbformat": 4,
 "nbformat_minor": 2
}
